src/arch/x64/interop/Memcpy.fst
@@ -1,0 +1,203 @@
+module Memcpy
+
+open LowStar.Buffer
+module B = LowStar.Buffer
+module BV = LowStar.BufferView
+open LowStar.Modifies
+module M = LowStar.Modifies
+open LowStar.ModifiesPat
+open FStar.HyperStack.ST
+module HS = FStar.HyperStack
+module S8 = SecretByte
+open Interop
+open Words_s
+open Types_s
+open X64.Machine_s
+open X64.Memory_i_s
+open X64.Vale.State_i
+open X64.Vale.Decls_i
+open BufferViewHelpers
+open Interop_assumptions
+#set-options "--z3rlimit 40"
+
+open Vale_memcpy
+
+#set-options "--initial_fuel 5 --max_fuel 5 --initial_ifuel 2 --max_ifuel 2"
+// TODO: Prove these two lemmas if they are not proven automatically
+let win_implies_pre (h0:HS.mem) (dst:s8) (src:s8)  (stack_b:b8) : Lemma
+  (requires pre_cond h0 dst src /\ B.length stack_b == 24 /\ live h0 stack_b /\ buf_disjoint_from stack_b [dst;src])
+  (ensures (
+B.length stack_b == 24 /\ live h0 stack_b /\ buf_disjoint_from stack_b [dst;src] /\ (  let taint_func (x:b8) : GTot taint =
+    if StrongExcludedMiddle.strong_excluded_middle (x == dst) then Secret else
+    if StrongExcludedMiddle.strong_excluded_middle (x == src) then Secret else
+    Public in
+  let buffers = stack_b::dst::src::[] in
+  let (mem:mem) = {addrs = addrs; ptrs = buffers; hs = h0} in
+  let addr_dst = addrs dst in
+  let addr_src = addrs src in
+  let addr_stack:nat64 = addrs stack_b + 0 in
+  let regs = fun r -> begin match r with
+    | Rsp -> addr_stack
+    | Rcx -> addr_dst
+    | Rdx -> addr_src
+    | _ -> init_regs r end in
+  let xmms = init_xmms in
+  let s0 = {ok = true; regs = regs; xmms = xmms; flags = 0; mem = mem; memTaint = create_valid_memtaint mem buffers taint_func} in
+  length_t_eq (TBase TUInt64) stack_b;
+  length_t_eq (TBase TUInt64) dst;
+  length_t_eq (TBase TUInt64) src;
+  va_pre (va_code_memcpy true) s0 true stack_b dst src ))) =
+  length_t_eq (TBase TUInt64) stack_b;
+  length_t_eq (TBase TUInt64) dst;
+  length_t_eq (TBase TUInt64) src;
+  assert(B.disjoint stack_b dst);
+  assert(B.disjoint stack_b src);
+  ()
+
+let win_implies_post (va_s0:va_state) (va_sM:va_state) (va_fM:va_fuel) (dst:s8) (src:s8)  (stack_b:b8) : Lemma
+  (requires pre_cond va_s0.mem.hs dst src /\ B.length stack_b == 24 /\ live va_s0.mem.hs stack_b /\ buf_disjoint_from stack_b [dst;src]/\
+    va_post (va_code_memcpy true) va_s0 va_sM va_fM true stack_b dst src )
+  (ensures post_cond va_s0.mem.hs va_sM.mem.hs dst src ) =
+  length_t_eq (TBase TUInt64) stack_b;
+  length_t_eq (TBase TUInt64) dst;
+  length_t_eq (TBase TUInt64) src;
+  ()
+
+val win_ghost_memcpy: dst:s8 -> src:s8 ->  stack_b:b8 -> (h0:HS.mem{pre_cond h0 dst src /\ B.length stack_b == 24 /\ live h0 stack_b /\ buf_disjoint_from stack_b [dst;src]}) -> GTot (h1:HS.mem{post_cond h0 h1 dst src })
+
+let win_ghost_memcpy dst src stack_b h0 =
+  let taint_func (x:b8) : GTot taint =
+    if StrongExcludedMiddle.strong_excluded_middle (x == dst) then Secret else
+    if StrongExcludedMiddle.strong_excluded_middle (x == src) then Secret else
+    Public in
+  let buffers = stack_b::dst::src::[] in
+  let (mem:mem) = {addrs = addrs; ptrs = buffers; hs = h0} in
+  let addr_dst = addrs dst in
+  let addr_src = addrs src in
+  let addr_stack:nat64 = addrs stack_b + 0 in
+  let regs = fun r -> begin match r with
+    | Rsp -> addr_stack
+    | Rcx -> addr_dst
+    | Rdx -> addr_src
+    | _ -> init_regs r end in
+  let xmms = init_xmms in
+  let s0 = {ok = true; regs = regs; xmms = xmms; flags = 0; mem = mem; memTaint = create_valid_memtaint mem buffers taint_func} in
+  length_t_eq (TBase TUInt64) stack_b;
+  length_t_eq (TBase TUInt64) dst;
+  length_t_eq (TBase TUInt64) src;
+  win_implies_pre h0 dst src stack_b ;
+  let s1, f1 = va_lemma_memcpy (va_code_memcpy true) s0 true stack_b dst src  in
+  // Ensures that the Vale execution was correct
+  assert(s1.ok);
+  // Ensures that the callee_saved registers are correct
+  assert(s0.regs Rbx == s1.regs Rbx);
+  assert(s0.regs Rbp == s1.regs Rbp);
+  assert(s0.regs Rdi == s1.regs Rdi);
+  assert(s0.regs Rsi == s1.regs Rsi);
+  assert(s0.regs Rsp == s1.regs Rsp);
+  assert(s0.regs R12 == s1.regs R12);
+  assert(s0.regs R13 == s1.regs R13);
+  assert(s0.regs R14 == s1.regs R14);
+  assert(s0.regs R15 == s1.regs R15);
+  assert(s0.xmms 6 == s1.xmms 6);
+  assert(s0.xmms 7 == s1.xmms 7);
+  assert(s0.xmms 8 == s1.xmms 8);
+  assert(s0.xmms 9 == s1.xmms 9);
+  assert(s0.xmms 10 == s1.xmms 10);
+  assert(s0.xmms 11 == s1.xmms 11);
+  assert(s0.xmms 12 == s1.xmms 12);
+  assert(s0.xmms 13 == s1.xmms 13);
+  assert(s0.xmms 14 == s1.xmms 14);
+  assert(s0.xmms 15 == s1.xmms 15);
+  // Ensures that va_code_memcpy is actually Vale code, and that s1 is the result of executing this code
+  assert (va_ensure_total (va_code_memcpy true) s0 s1 f1);
+  win_implies_post s0 s1 f1 dst src stack_b ;
+  s1.mem.hs
+
+// TODO: Prove these two lemmas if they are not proven automatically
+let lin_implies_pre (h0:HS.mem) (dst:s8) (src:s8)  (stack_b:b8) : Lemma
+  (requires pre_cond h0 dst src /\ B.length stack_b == 24 /\ live h0 stack_b /\ buf_disjoint_from stack_b [dst;src])
+  (ensures (
+B.length stack_b == 24 /\ live h0 stack_b /\ buf_disjoint_from stack_b [dst;src] /\ (  let taint_func (x:b8) : GTot taint =
+    if StrongExcludedMiddle.strong_excluded_middle (x == dst) then Secret else
+    if StrongExcludedMiddle.strong_excluded_middle (x == src) then Secret else
+    Public in
+  let buffers = stack_b::dst::src::[] in
+  let (mem:mem) = {addrs = addrs; ptrs = buffers; hs = h0} in
+  let addr_dst = addrs dst in
+  let addr_src = addrs src in
+  let addr_stack:nat64 = addrs stack_b + 0 in
+  let regs = fun r -> begin match r with
+    | Rsp -> addr_stack
+    | Rdi -> addr_dst
+    | Rsi -> addr_src
+    | _ -> init_regs r end in
+  let xmms = init_xmms in
+  let s0 = {ok = true; regs = regs; xmms = xmms; flags = 0; mem = mem; memTaint = create_valid_memtaint mem buffers taint_func} in
+  length_t_eq (TBase TUInt64) stack_b;
+  length_t_eq (TBase TUInt64) dst;
+  length_t_eq (TBase TUInt64) src;
+  va_pre (va_code_memcpy false) s0 false stack_b dst src ))) =
+  length_t_eq (TBase TUInt64) stack_b;
+  length_t_eq (TBase TUInt64) dst;
+  length_t_eq (TBase TUInt64) src;
+  assert(B.disjoint stack_b dst);
+  assert(B.disjoint stack_b src);
+  ()
+
+let lin_implies_post (va_s0:va_state) (va_sM:va_state) (va_fM:va_fuel) (dst:s8) (src:s8)  (stack_b:b8) : Lemma
+  (requires pre_cond va_s0.mem.hs dst src /\ B.length stack_b == 24 /\ live va_s0.mem.hs stack_b /\ buf_disjoint_from stack_b [dst;src]/\
+    va_post (va_code_memcpy false) va_s0 va_sM va_fM false stack_b dst src )
+  (ensures post_cond va_s0.mem.hs va_sM.mem.hs dst src ) =
+  length_t_eq (TBase TUInt64) stack_b;
+  length_t_eq (TBase TUInt64) dst;
+  length_t_eq (TBase TUInt64) src;
+  ()
+
+val lin_ghost_memcpy: dst:s8 -> src:s8 ->  stack_b:b8 -> (h0:HS.mem{pre_cond h0 dst src /\ B.length stack_b == 24 /\ live h0 stack_b /\ buf_disjoint_from stack_b [dst;src]}) -> GTot (h1:HS.mem{post_cond h0 h1 dst src })
+
+let lin_ghost_memcpy dst src stack_b h0 =
+  let taint_func (x:b8) : GTot taint =
+    if StrongExcludedMiddle.strong_excluded_middle (x == dst) then Secret else
+    if StrongExcludedMiddle.strong_excluded_middle (x == src) then Secret else
+    Public in
+  let buffers = stack_b::dst::src::[] in
+  let (mem:mem) = {addrs = addrs; ptrs = buffers; hs = h0} in
+  let addr_dst = addrs dst in
+  let addr_src = addrs src in
+  let addr_stack:nat64 = addrs stack_b + 0 in
+  let regs = fun r -> begin match r with
+    | Rsp -> addr_stack
+    | Rdi -> addr_dst
+    | Rsi -> addr_src
+    | _ -> init_regs r end in
+  let xmms = init_xmms in
+  let s0 = {ok = true; regs = regs; xmms = xmms; flags = 0; mem = mem; memTaint = create_valid_memtaint mem buffers taint_func} in
+  length_t_eq (TBase TUInt64) stack_b;
+  length_t_eq (TBase TUInt64) dst;
+  length_t_eq (TBase TUInt64) src;
+  lin_implies_pre h0 dst src stack_b ;
+  let s1, f1 = va_lemma_memcpy (va_code_memcpy false) s0 false stack_b dst src  in
+  // Ensures that the Vale execution was correct
+  assert(s1.ok);
+  // Ensures that the callee_saved registers are correct
+  assert(s0.regs Rbx == s1.regs Rbx);
+  assert(s0.regs Rbp == s1.regs Rbp);
+  assert(s0.regs R12 == s1.regs R12);
+  assert(s0.regs R13 == s1.regs R13);
+  assert(s0.regs R14 == s1.regs R14);
+  assert(s0.regs R15 == s1.regs R15);
+  // Ensures that va_code_memcpy is actually Vale code, and that s1 is the result of executing this code
+  assert (va_ensure_total (va_code_memcpy false) s0 s1 f1);
+  lin_implies_post s0 s1 f1 dst src stack_b ;
+  s1.mem.hs
+
+let ghost_memcpy dst src stack_b h0 =
+  if win then win_ghost_memcpy dst src stack_b h0
+  else lin_ghost_memcpy dst src stack_b h0
+
+let memcpy dst src  =
+  push_frame();
+  let (stack_b:b8) = B.alloca (UInt8.uint_to_t 0) (UInt32.uint_to_t 24) in
+  st_put (fun h -> pre_cond h dst src /\ B.length stack_b == 24 /\ live h stack_b /\ buf_disjoint_from stack_b [dst;src]) (ghost_memcpy dst src stack_b);
+  pop_frame()
